\begin{exercice}
Résoudre les équations suivantes :
\begin{multicols}{3}
\begin{enumerate} 
\item ${{4}^{x}}=0,0625$
\item $4\cdot {{2}^{x}}=0,25$
\item ${{144}^{x}}=2\sqrt{3}$
\item $\sqrt{{{8}^{x}}}=0,125$
\item ${{\left( \frac{1}{64} \right)}^{x}}=4'096$
\item $2\cdot {{\left( 1,07 \right)}^{x}}=3\cdot {{\left( 1,05 \right)}^{x}}$	
\item ${{54}^{x+1}}=\frac{\sqrt[3]{4}}{6}$
\item $\sqrt[x+1]{4}=\sqrt[3x-1]{16}$
\item $\frac{10'206}{{{3}^{x+3}}}=14$
\item $\sqrt{{{3}^{3x+2}}}=59'049$
\item $\sqrt[5]{{{4}^{2x+1}}}=2,3$
\item ${{3}^{\sqrt{x}}}=243$
\end{enumerate}
\end{multicols}
\end{exercice}

\begin{exercice}
Résoudre les équations logarithmiques suivantes :
\begin{multicols}{2}
\begin{enumerate}
\item $\log \left( 3x-5 \right)=0$
\item $\log \left( 6-x \right)=1$
\item $\log \left( 3x+7 \right)=2\log \left( 2 \right)$
\item $\log \left( x+3 \right)+\log \left( x+5 \right)=\log \left( 15 \right)$
\item $\log \left( x-2 \right)+\log \left( x+2 \right)=\log \left( 45 \right)$
\item $2\log \left( x-4 \right)=\log \left( x \right)-2\log \left( 2 \right)$
\item $\log \left( 4x+1 \right)+\log \left( x+2 \right)-2\log \left( 3x \right)=0$
\item $\log \left( {{x}^{2}}+2x-3 \right)-2\log \left( x-1 \right)=2$
\item $\log \left( -x-2 \right)=\log \left( \frac{-x-11}{x+3} \right)$
\item $\log \left( x+2 \right)=\log \left( -x-11 \right)-\log \left( x+3 \right)$
\end{enumerate}
\end{multicols}
\end{exercice}