\begin{solution}
Calculer les limites suivantes :
\begin{enumerate}
\item $\underset{x\to 0}{\mathop{\lim }}\,\frac{{{x}^{3}}-3{{x}^{2}}+2x-2}{-{{x}^{2}}+3x+2}=-1$
\item $\underset{x\to 2}{\mathop{\lim }}\,\left( 2{{x}^{2}}+4x-5 \right)=11$
\item $\underset{x\to -3}{\mathop{\lim }}\,\frac{2x-1}{{{x}^{2}}}=-\frac{7}{9}$
\item $\underset{x\to -1}{\mathop{\lim }}\,\frac{{{x}^{3}}-3{{x}^{2}}+4}{3{{x}^{3}}-18{{x}^{2}}+36x-24}=\left[ \frac{0}{\alpha } \right]=0$
\end{enumerate}
\end{solution}

\begin{solution}
Calculer les limites suivantes :
\begin{enumerate}
\item $\underset{x\to 1}{\mathop{\lim }}\,\frac{{{x}^{3}}+2{{x}^{2}}-x-2}{{{x}^{2}}+x-2}=\left[ \frac{0}{0} \right]=\underset{x\to 1}{\mathop{\lim }}\,\frac{\left( x-1 \right)\left( {{x}^{2}}+3x+2 \right)}{\left( x-1 \right)\left( x+2 \right)}=\underset{x\to 1}{\mathop{\lim }}\,\frac{{{x}^{2}}+3x+2}{x+2}=\frac{6}{3}=2$
\item $\underset{x\to 1}{\mathop{\lim }}\,\frac{{{x}^{3}}-3x+2}{{{x}^{2}}-6x+5}=\left[ \frac{0}{0} \right]=\underset{x\to 1}{\mathop{\lim }}\,\frac{\left( x-1 \right)\left( {{x}^{2}}+x-2 \right)}{\left( x-1 \right)\left( x-5 \right)}=\underset{x\to 1}{\mathop{\lim }}\,\frac{{{x}^{2}}+x-2}{x-5}=\frac{0}{-4}=0$	
\item $\underset{x\to 5}{\mathop{\lim }}\,\frac{{{x}^{3}}-3x+2}{{{x}^{2}}-6x+5}=\left[ \frac{\alpha }{0} \right]=\pm \infty \begin{matrix}
   \nearrow   \\
   \searrow   \\
\end{matrix}\begin{matrix}
   \underset{x<5}{\mathop{\underset{x\to 5}{\mathop{\lim }}\,}}\,\frac{{{x}^{3}}-3x+2}{{{x}^{2}}-6x+5}=-\infty   \\
   \underset{x>5}{\mathop{\underset{x\to 5}{\mathop{\lim }}\,}}\,\frac{{{x}^{3}}-3x+2}{{{x}^{2}}-6x+5}=+\infty   \\
\end{matrix}\text{               }a.v.\text{ }x=5$	
\item $\begin{array}{ll}
  & \underset{x\to 2}{\mathop{\lim }}\,\frac{{{x}^{3}}-3{{x}^{2}}+4}{3{{x}^{3}}-18{{x}^{2}}+36x-24}=\left[ \frac{0}{0} \right]=\underset{x\to 2}{\mathop{\lim }}\,\frac{{{\left( x-2 \right)}^{2}}\left( x+1 \right)}{3{{\left( x-2 \right)}^{3}}}= \\ 
 & \underset{x\to 2}{\mathop{\lim }}\,\frac{x+1}{3\left( x-2 \right)}=\pm \infty \begin{matrix}
   \nearrow   \\
   \searrow   \\
\end{matrix}\begin{matrix}
   \underset{x<2}{\mathop{\underset{x\to 2}{\mathop{\lim }}\,}}\,\frac{x+1}{3\left( x-2 \right)}=-\infty   \\
   \underset{x>2}{\mathop{\underset{x\to 2}{\mathop{\lim }}\,}}\,\frac{x+1}{3\left( x-2 \right)}=+\infty   \\
\end{matrix}\text{             }a.v.\text{ }x=2 \\ 
\end{array} $
\item $\underset{x\to \frac{1}{2}}{\mathop{\lim }}\,\frac{8{{x}^{3}}+2{{x}^{2}}-5x+1}{8{{x}^{3}}+10{{x}^{2}}-11x+2}=\left[ \frac{0}{0} \right]=\underset{x\to \frac{1}{2}}{\mathop{\lim }}\,\frac{\left( 2x-1 \right)\left( 4x-1 \right)\left( x+1 \right)}{\left( 2x-1 \right)\left( 4x-1 \right)\left( x+2 \right)}=\underset{x\to \frac{1}{2}}{\mathop{\lim }}\,\frac{x+1}{x+2}=\frac{3}{5}$
\item $\underset{x\to \frac{1}{4}}{\mathop{\lim }}\,\frac{8{{x}^{3}}+2{{x}^{2}}-5x+1}{8{{x}^{3}}+10{{x}^{2}}-11x+2}=\left[ \frac{0}{0} \right]=\underset{x\to \frac{1}{4}}{\mathop{\lim }}\,\frac{\left( 2x-1 \right)\left( 4x-1 \right)\left( x+1 \right)}{\left( 2x-1 \right)\left( 4x-1 \right)\left( x+2 \right)}=\underset{x\to \frac{1}{4}}{\mathop{\lim }}\,\frac{x+1}{x+2}=\frac{5}{9}$
\item $\underset{x\to 1}{\mathop{\lim }}\,\frac{{{x}^{4}}-2{{x}^{3}}+2{{x}^{2}}-2x+1}{{{x}^{4}}-2{{x}^{3}}+{{x}^{2}}}=\left[ \frac{0}{0} \right]=\underset{x\to 1}{\mathop{\lim }}\,\frac{{{\left( x-1 \right)}^{2}}\left( {{x}^{2}}+1 \right)}{{{x}^{2}}{{\left( x-1 \right)}^{2}}}=\underset{x\to 1}{\mathop{\lim }}\,\frac{{{x}^{2}}+1}{{{x}^{2}}}=2$
\item $\underset{x\to 0}{\mathop{\lim }}\,\frac{{{x}^{4}}-2{{x}^{3}}+2{{x}^{2}}-2x+1}{{{x}^{4}}-2{{x}^{3}}+{{x}^{2}}}=\left[ \frac{\alpha }{0} \right]=+\infty $ 	a.v. $x=0$  
(la réponse $-\infty $est refusée car le dénominateur est > 0) 

\item $\underset{{}}{\mathop{\underset{x\to 0}{\mathop{\lim }}\,}}\,\frac{{{x}^{4}}-5{{x}^{3}}+6{{x}^{2}}+4x-8}{{{x}^{3}}-4{{x}^{2}}+4x}=\pm \infty \begin{matrix}
   \nearrow   \\
   \searrow   \\
\end{matrix}\begin{matrix}
   \underset{x<0}{\mathop{\underset{x\to 0}{\mathop{\lim }}\,}}\,\frac{{{x}^{4}}-5{{x}^{3}}+6{{x}^{2}}+4x-8}{{{x}^{3}}-4{{x}^{2}}+4x}=+\infty   \\
   \underset{x>0}{\mathop{\underset{x\to 0}{\mathop{\lim }}\,}}\,\frac{{{x}^{4}}-5{{x}^{3}}+6{{x}^{2}}+4x-8}{{{x}^{3}}-4{{x}^{2}}+4x}=-\infty   \\
\end{matrix}\text{         }a.v.\text{ }x=0$
$\underset{x\to -2}{\mathop{\lim }}\,\frac{{{x}^{4}}-8{{x}^{2}}+16}{{{x}^{3}}+2{{x}^{2}}-4x-8}=\underset{x\to -2}{\mathop{\lim }}\,\frac{{{\left( x-2 \right)}^{2}}{{\left( x+2 \right)}^{2}}}{{{\left( x+2 \right)}^{2}}\left( x-2 \right)}=\underset{x\to -2}{\mathop{\lim }}\,\left( x-2 \right)=-4$
\end{enumerate}
\end{solution}

\begin{solution}
Calculer les limites suivantes :
\begin{enumerate}
\item $\underset{x\to \pm \infty }{\mathop{\lim }}\,\left( 3{{x}^{2}}-5x-4 \right)=+\infty $
\item $\underset{x\to \pm \infty }{\mathop{\lim }}\,\left( 2{{x}^{3}}-8{{x}^{2}}+4x+7 \right)=\pm \infty $
\item $\underset{x\to \pm \infty }{\mathop{\lim }}\,\left( -{{x}^{2}}+1 \right)=-\infty $
\item $\underset{x\to \pm \infty }{\mathop{\lim }}\,\left( -2{{x}^{5}}+{{x}^{4}}+4{{x}^{3}}+3{{x}^{2}}-5 \right)=\mp \infty $
\item $\underset{x\to \pm \infty }{\mathop{\lim }}\,\frac{{{x}^{3}}+2{{x}^{2}}-2}{{{x}^{2}}+x-3}=\pm \infty $
\item $\underset{x\to \pm \infty }{\mathop{\lim }}\,\frac{-2{{x}^{3}}+{{x}^{2}}-1}{5{{x}^{2}}-3x+4}=\mp \infty $
\item $\underset{x\to \pm \infty }{\mathop{\lim }}\,\frac{5{{x}^{3}}+{{x}^{2}}+4x+7}{5{{x}^{3}}+3{{x}^{2}}-x+4}=1\text{  }a.h.\text{ }y=1$
\item $\underset{x\to \pm \infty }{\mathop{\lim }}\,\frac{{{x}^{2}}+2x-4}{{{x}^{3}}-x+5}=0\text{  }a.h.\text{ }y=0$
\item $\underset{x\to \pm \infty }{\mathop{\lim }}\,\frac{2{{x}^{4}}+{{x}^{3}}-5{{x}^{2}}-2x+3}{5{{x}^{4}}+3{{x}^{3}}-{{x}^{2}}+x+7}=\frac{2}{5}\text{  }a.h.\text{ }y=\frac{2}{5}$
\item $\underset{x\to \pm \infty }{\mathop{\lim }}\,\frac{-2{{x}^{3}}-4{{x}^{2}}+1}{3{{x}^{3}}-5{{x}^{2}}+2x-7}=-\frac{2}{3}\text{  }a.h.\text{ }y=-\frac{2}{3}$
\item $\underset{x\to \pm \infty }{\mathop{\lim }}\,\frac{-{{x}^{4}}+2{{x}^{3}}-5{{x}^{2}}-2x+1}{{{x}^{3}}+{{x}^{2}}-3}=\mp \infty $
\item $\underset{x\to \pm \infty }{\mathop{\lim }}\,\frac{1}{{{x}^{2}}}=0\text{  }a.h.\text{ }y=0$
\end{enumerate}
\end{solution}